src/examples/bank.v
@@ -1,0 +1,413 @@
+From iris.proofmode Require Import tactics.
+From iris.bi Require Import monpred.
+From iris.program_logic Require weakestpre.
+From iris.algebra Require Import gmap.
+
+From self.base Require Import primitive_laws.
+From self.lang Require Import lang.
+From self.high Require Import dprop.
+
+From self.lang Require Export notation lang lemmas tactics syntax.
+From self.algebra Require Import view.
+From self.base Require Import primitive_laws class_instances adequacy.
+From self.high Require Import proofmode wpc_proofmode.
+From self.high Require Import weakestpre_exp weakestpre_at weakestpre_na locations.
+From self.high.modalities Require Import fence.
+From self.high Require Import protocol no_buffer abstract_state_instances.
+
+Section FAA_Axiom.
+  Context `{AbstractState ST}.
+  Context `{!nvmG Σ}.
+
+  Implicit Types (ℓ : loc) (s : ST) (prot : LocationProtocol ST).
+
+  Definition faa: expr :=
+    rec: "faa" "l" "v_add" :=
+      let: "v_old" := !_AT "l" in
+      if: (CAS "l" "v_old" ("v_old" + "v_add")) then
+        "v_old"
+      else
+        "faa" "l" "v_add".
+
+  Lemma wp_faa Q R next ℓ prot `{!ProtocolConditions prot} ss (v_add: Z) st E:
+    {{{
+      ℓ ↦_AT^{prot} (ss) ∗
+      (∀ s_l (v_l: Z) s_p v_p, ∃ P,
+        (  (* The state we write fits in the history. *)
+           (<obj> (prot.(p_full) s_l #v_l -∗ ⌜ s_l ⊑ next s_l ⌝)) ∗
+           (∀ s_n v_n, ⌜ s_l ⊑ s_n ⌝ -∗ prot.(p_full) s_l #v_l -∗
+                       prot.(p_full) s_n v_n ∨
+                         (prot.(p_read) s_n v_n ∧
+                          ∃ s_n' v_n', ⌜ s_n ⊑ s_n' ⌝ ∗ prot.(p_full) s_n' v_n') -∗
+                       ⌜ next s_l ⊑ s_n ⌝) ∗
+           (* Extract the objective knowledge from [p_pers] *)
+           (<obj> (prot.(p_pers) s_p v_p -∗ <obj> P ∗ (P -∗ prot.(p_pers) s_p v_p))) ∗
+           (* Extract from the location we load. *)
+           (<obj> (prot.(p_full) s_l #v_l ∗ P -∗ prot.(p_read) s_l #v_l ∗ R s_l v_l)) ∗
+           (* Establish the invariant for the value we store. *)
+           (R s_l v_l ==∗ prot.(p_full) (next s_l) #(v_l + v_add) ∗ <obj> P ∗ Q s_l v_l)
+        ))
+    }}}
+      FAA #ℓ #v_add @ st; E
+    {{{ (v_l: Z) s_l, RET #v_l;
+        <fence> Q s_l v_l ∗ ℓ ↦_AT^{prot} (ss ++ [next s_l])
+    }}}.
+    Proof.
+  Admitted.
+End FAA_Axiom.
+
+Section Bank.
+  Context `{!nvmG Σ}.
+
+  Variables (ℓ: loc) (γ: gname).
+
+  (* axiomatized section begins *)
+  Definition trans := (gmap nat nat) → (gmap nat nat).
+  Definition promise := trans → Prop.
+  Variables (nextgen: dProp Σ → dProp Σ) (token: gname → promise → iProp Σ) (rely: gname → promise → iProp Σ).
+
+  Instance rely_persistent prom: Persistent (rely γ prom).
+  Proof. Admitted.
+
+  Hypothesis (token_strengthen: ∀ (prom1 prom2: promise), (∀ tr, prom2 tr → prom1 tr) → token γ prom1 ==∗ token γ prom2).
+  Hypothesis (token_bupd_rely: ∀ (prom: promise), token γ prom ==∗ token γ prom ∗ rely γ prom).
+  Hypothesis (rely_weaken: ∀ (prom1 prom2: promise), (∀ tr, prom1 tr → prom2 tr) → rely γ prom1 -∗ rely γ prom2).
+  (* axiomatized section ends *)
+
+  Definition deposit: expr :=
+    λ: "n",
+      FAA #ℓ "n" ;;
+      Flush #ℓ ;;
+      FenceSync.
+
+  Definition withdraw: expr :=
+    λ: "n",
+      let: "v" := FAA #ℓ (- "n") in
+      (* Flush #ℓ ;; *)
+      (* FenceSync ;; *)
+      "v".
+
+  (* abstract state *)
+  Program Instance list_abstract_state T `{!EqDecision T, Countable T} : AbstractState (list T) :=
+    { abs_state_relation := prefix }.
+
+  Notation state := (list (nat + nat)).
+
+  (* ghost resource *)
+  Context `{!ghost_mapG Σ nat nat}.
+
+  Definition to_auth (h: state): gmap nat nat :=
+    omap (λ x, match x with inl n => Some n | _ => None end) $ map_seq 0 h.
+
+  Notation dsum h :=
+    (foldl (λ sum x, match x with inl n => sum + n | _ => sum end) 0 h).
+
+  Notation wsum h :=
+    (foldl (λ sum x, match x with inr n => sum + n | _ => sum end) 0 h).
+
+  Definition state_match h v: dProp Σ :=
+    ⌜ ∃ (n: nat), #n = v ∧ (wsum h + n)%nat = dsum h ⌝.
+
+  Definition full_pred h: iProp Σ :=
+    ghost_map_auth γ (DfracOwn 1) (to_auth h) ∗
+    ∃ (m__w: gmap nat nat), ([∗ map] k ↦ n ∈ m__w, ghost_map_elem γ k (DfracOwn 1) n) ∗
+                          ⌜ wsum h = [^(Nat.add) map] n ∈ m__w, n ⌝.
+
+  Definition map_trans k (m: gmap nat nat) :=
+    filter (λ '(k', _), k' ≤ k) m.
+
+  Definition map_prom k tr :=
+    ∃ k', k' ≥ k ∧ tr = map_trans k'.
+
+  (* protocol for [ℓ] *)
+  Definition prot : LocationProtocol state :=
+    {| p_full := λ (h : state) v, (state_match h v ∗ ⎡ full_pred h ⎤ )%I;
+      p_read := λ (h : state) v, state_match h v;
+      p_pers := λ (h : state) v, ⎡ token γ (map_prom (length h - 1)) ⎤%I;
+      p_bumper h := h |}.
+  Global Instance prot_cond : ProtocolConditions prot.
+  Proof.
+    split; try done; try solve_proper; try apply _.
+    - intros.
+      rewrite /prot /=.
+      rewrite bi.equiv_entails.
+      split.
+      { iIntros "[% ?]". iFrame "∗%". done. }
+      { iIntros "[% H]". iFrame "%".
+        iDestruct ("H" with "[//]") as "[_ $]". }
+    - rewrite /prot /=.
+      iIntros (??) "token".
+      admit.
+    - iIntros.
+      iApply post_crash_flush_pure.
+      done.
+  Admitted.
+
+  Definition is_bank: dProp Σ := ℓ ↦_AT^{prot} [ [] ].
+  Definition receipt (n: nat): dProp Σ := ⎡ ∃ k, ghost_map_elem γ k (DfracOwn 1) n ∗ rely γ (map_prom k) ⎤.
+
+  (* auxiliary lemmas *)
+
+  Lemma to_auth_lookup_length_None h:
+    to_auth h !! length h = None.
+  Proof.
+    rewrite /to_auth.
+    rewrite lookup_omap.
+    rewrite bind_None.
+    left.
+    rewrite lookup_map_seq_None.
+    lia.
+  Qed.
+
+  Lemma to_auth_snoc_insert h n:
+    <[ length h := n ]> (to_auth h) = to_auth (h ++ [inl n]).
+  Proof.
+    rewrite {2}/to_auth map_seq_snoc (omap_insert_Some _ _ _ _ n); last done.
+    f_equal.
+  Qed.
+
+  Lemma to_auth_snoc_noop h n:
+    to_auth h = to_auth (h ++ [inr n]).
+  Proof.
+    rewrite {2}/to_auth map_seq_snoc omap_insert_None /=; last done.
+    rewrite -omap_delete delete_notin; last (apply lookup_map_seq_None; lia).
+    done.
+    Qed.
+
+  Lemma to_auth_dsum h:
+    dsum h = [^Nat.add map] n ∈ to_auth h, n.
+  Proof.
+    induction h  as [ | [ n | n ] h IH ] using rev_ind.
+    - rewrite /to_auth omap_empty big_opM_empty //.
+    - rewrite -to_auth_snoc_insert foldl_snoc.
+      rewrite big_opM_insert; last apply to_auth_lookup_length_None.
+      lia.
+    - rewrite -to_auth_snoc_noop foldl_snoc.
+      lia.
+  Qed.
+
+  Lemma full_pred_deposit_bupd n h:
+    full_pred h ==∗ full_pred (h ++ [inl n]) ∗ ghost_map_elem γ (length h) (DfracOwn 1) n.
+  Proof.
+    rewrite /full_pred.
+    iIntros "[auth (% & tokens & %)]".
+    iMod (ghost_map_insert (length h) n with "auth") as "[auth $]".
+    { apply to_auth_lookup_length_None. }
+    rewrite to_auth_snoc_insert.
+    iFrame "auth".
+    iModIntro.
+    iExists m__w.
+    iFrame.
+    rewrite foldl_snoc //.
+  Qed.
+
+  Lemma full_pred_withdraw n (v: nat) h:
+    state_match h #v -∗ ⎡ full_pred h ⎤ -∗ receipt n -∗ ⎡ full_pred (h ++ [inr n]) ⎤ ∗ ⌜ n ≤ v ⌝.
+  Proof.
+    rewrite /full_pred -to_auth_snoc_noop.
+    iIntros "%steq [auth (% & tokens & %eq)] (%k & frag & _)".
+    simplify_eq.
+    rewrite embed_big_sepM.
+    iAssert ⌜ m__w !! k = None ⌝%I as "%".
+    { destruct ((m__w !! k)) as [ | ] eqn:?; last done.
+      iPoseProof (big_sepM_lookup _ _ k with "tokens") as "frag'"; first done.
+      iPoseProof (ghost_map_elem_valid_2 with "[$] [$]") as "[% _]".
+      done. }
+    iPoseProof (big_sepM_insert with "[$tokens $frag]") as "tokens"; first done.
+    rewrite -embed_big_sepM.
+    iPoseProof (ghost_map_lookup_big with "[$] [$]") as "%".
+    iFrame.
+    iSplit.
+    { iExists (<[ k := n ]> m__w).
+      iFrame.
+      iPureIntro.
+      rewrite foldl_snoc /=.
+      rewrite big_opM_insert; last done.
+      lia. }
+    pose proof (to_auth_dsum h) as bigeq.
+    rewrite -(map_difference_union (<[k:=n]> m__w) (to_auth h)) in bigeq; last done.
+    rewrite big_opM_union in bigeq; last by apply map_disjoint_difference_r.
+    iPureIntro.
+    rewrite big_opM_insert in bigeq; last done.
+    destruct steq as (? & ? & ?).
+    simplify_eq.
+    lia.
+  Qed.
+
+  Lemma map_prom_strengthen k1 k2:
+    k1 ≤ k2 → ∀ tr, map_prom k2 tr → map_prom k1 tr.
+  Proof.
+    rewrite /map_prom.
+    intros ??(k' & ? & ?).
+    exists k'.
+    split; last done.
+    lia.
+  Qed.
+
+  Lemma wp_deposit n:
+    {{{ is_bank }}}
+      deposit #n
+    {{{ RET #(); receipt n }}}.
+  Proof.
+    rewrite /is_bank.
+    iIntros (?) "#is_bank HΦ".
+    wp_pures.
+    wp_bind (FAA _ _).
+    iApply (wp_faa
+              (λ h _, ⎡ ghost_map_elem γ (length h) (DfracOwn 1) n⎤)%I
+              (λ h v, state_match h #v ∗ ⎡ full_pred h ⎤)%I
+              (λ h, h ++ [inl n]) _ prot).
+    { iSplitL; first iFrame "#".
+      iIntros.
+      iExists (True)%I.
+      iSplitL "".
+      { iIntros "!> _".
+        iPureIntro.
+        by eexists. }
+      iSplitL "".
+      { iIntros (???) "[_ [full1 _]] [[_ [full2 _]] | [_ (% & % & % & [_ [full2 _]])]]";
+          by iPoseProof (ghost_map_auth_valid_2 with "full1 full2") as "[%frac _]". }
+      iSplitL "".
+      { iIntros "!> pers".
+        iSplitL ""; first by iModIntro.
+        iIntros. iFrame. }
+      iSplitL "".
+      { iIntros "!> [full _]".
+        iSplit.
+        - iDestruct "full" as "[? _]".
+          done.
+        - iFrame. }
+      iIntros "[%steq full]".
+      iMod (full_pred_deposit_bupd n with "full") as "[full receipt]".
+      iModIntro.
+      iFrame.
+      iSplitPure.
+      { rewrite ?foldl_snoc.
+        destruct steq as (?n' & ? & ?).
+        simplify_eq.
+        exists (n' + n).
+        split; first rewrite Nat2Z.inj_add //.
+        lia. }
+      by iModIntro.
+    }
+    iModIntro.
+    iIntros (??) "[frag #mapsto]".
+    iPoseProof (post_fence_flush_free with "frag") as "frag".
+    wp_pures.
+    wp_bind (Flush _).
+    iPoseProof (mapsto_at_store_lb with "mapsto") as "#lb".
+    iApply (weakestpre_exp.wp_flush_lb _ _ _ _ _ ⎡ rely γ (map_prom $ length s_l) ⎤%I with "[$lb]").
+    { iSplit.
+      { iDestruct "is_bank" as (???????) "H".
+        iNamed "H".
+        iAssumption. }
+      iIntros "!>" (???).
+      iExists (True)%I.
+      iSplit; first by iIntros "_ !>!>".
+      iIntros "_".
+      rewrite /p_pers /prot //=.
+      iSplit.
+      - iIntros "[% %eq] pers".
+        iMod (token_strengthen _ (map_prom (length s_l)) with "pers").
+        { apply map_prom_strengthen.
+          assert (length_eq: length s_l + length [@inl nat nat n] = length s_p + length k).
+          { rewrite -?app_length. by f_equiv. }
+          simpl in length_eq.
+          lia. }
+        rewrite app_length //=.
+        replace (_ + 1 - 1) with (length s_l) by lia.
+        iMod (token_bupd_rely with "[$]") as "[? ?]".
+        by iFrame.
+      - iIntros "[% ->] pers".
+        iMod (token_bupd_rely with "[$]") as "[$ rely]".
+        iModIntro.
+        iApply (rely_weaken with "rely").
+        apply map_prom_strengthen.
+        rewrite ?app_length //=.
+        lia.
+    }
+    iIntros "!> post_fence_sync".
+    wp_pures.
+    iApply (weakestpre_exp.wp_fence_sync _ prot with "post_fence_sync").
+    iIntros "!> [_ rely]".
+    iApply "HΦ".
+    iExists (length s_l).
+    iFrame.
+  Qed.
+
+  Lemma wp_withdraw n:
+    {{{ is_bank ∗ receipt n }}}
+      withdraw #n
+    {{{ (v: Z), RET #v; ⌜ (0 ≤ v)%Z ⌝ }}}.
+  Proof.
+    rewrite /is_bank.
+    iIntros (?) "[#is_bank receipt] HΦ".
+    wp_pures.
+    wp_bind (FAA _ _).
+    iApply (wp_faa
+              (λ h v, state_match h #v)%I
+              (λ h v, state_match h #v ∗ ⎡ full_pred h ⎤)%I
+              (λ h, h ++ [inr n]) _ prot with "[receipt]").
+    { iSplitL ""; first iFrame "#".
+      iIntros.
+      iExists (True)%I.
+      iSplitL "".
+      { iIntros "!> _".
+        iPureIntro.
+        by eexists. }
+      iSplitL "".
+      { iIntros (???) "[_ [full1 _]] [[_ [full2 _]] | [_ (% & % & % & [_ [full2 _]])]]";
+          by iPoseProof (ghost_map_auth_valid_2 with "full1 full2") as "[%frac _]". }
+      iSplitL "".
+      { iIntros "!> pers".
+        iSplitL ""; first by iModIntro.
+        iIntros. iFrame. }
+      iSplitL "".
+      { iIntros "!> [full _]".
+        iSplit.
+        - iDestruct "full" as "[? _]".
+          done.
+        - iFrame. }
+      iIntros "[%eq full]".
+      destruct eq as (n' & ? & ?).
+      simplify_eq.
+      iPoseProof (full_pred_withdraw with "[%] full receipt") as "[full %]".
+      { by exists n'. }
+      iFrame "%".
+      iModIntro.
+      iFrame.
+      rewrite Z.add_opp_r.
+      iSplit.
+      { iPureIntro.
+        rewrite -Nat2Z.inj_sub; last done.
+        eexists.
+        split; first done.
+        rewrite ?foldl_snoc.
+        lia. }
+      iSplit; first by iModIntro.
+      iPureIntro.
+      by eexists.
+    }
+    iIntros "!>" (??) "[post #mapsto]".
+    iPoseProof (post_fence_flush_free with "post") as "(% & % & %)".
+    wp_pures.
+    iModIntro.
+    iApply "HΦ".
+    simplify_eq.
+    iPureIntro.
+    lia.
+  Qed.
+
+  Lemma receipt_nextgen n:
+    receipt n ⊢ nextgen $ receipt n.
+  Proof. Abort.
+
+  Lemma is_bank_nextgen:
+    is_bank ⊢ nextgen is_bank.
+  Proof. Abort.
+
+  Lemma receipt_split n1 n2:
+    receipt n1 ∗ receipt n2 ⊣⊢ receipt (n1 + n2).
+  Proof. Abort.
+
+End Bank.
